verif/trie/verif/verif_key.v
@@ -1,0 +1,70 @@
+(** * verif_key.v: Correctness proof of key *)
+Require Import VST.floyd.proofauto.
+Require Import VST.floyd.library.
+
+Require Import DB.common.
+Require Import DB.tactics.
+
+Require Import DB.functional.keyslice.
+
+Require Import DB.representation.string.
+Require Import DB.representation.key.
+
+Require Import DB.specs.
+
+Import Coq.Lists.List.ListNotations.
+
+Definition Gprog : funspecs :=
+  ltac:(with_library prog [
+        surely_malloc_spec; (* KV_NewKey_spec; *)
+        KV_MoveKey_spec; KV_GetCharArray_spec;
+        KV_GetCharArraySize_spec
+       ]).
+
+Lemma body_KV_MoveKey: semax_body Vprog Gprog f_KV_MoveKey KV_MoveKey_spec.
+Proof.
+  start_function.
+  forward.
+  forward_if (True);
+    [
+      unfold cstring_len;
+      forward_if (True);
+      [forward; entailer! | assert_PROP (False) by entailer!; contradiction] |
+      forward; entailer! |
+    ].
+  forward_call (tkey).
+  split3; auto; simpl; rep_omega.
+  Intros k.
+  forward.
+  elim_cast_pointer.
+  forward.
+  forward.
+  Exists k.
+  Exists s.
+  fold_keyrep.
+  entailer!.
+Qed.
+
+Lemma body_KV_GetCharArray: semax_body Vprog Gprog f_KV_GetCharArray KV_GetCharArray_spec.
+Proof.
+  start_function.
+  unfold key_rep.
+  Intros.
+  forward_if (True); [forward; entailer! | assert_PROP (False) by entailer!; contradiction | ].
+  forward.
+  forward.
+  fold_keyrep.
+  entailer!.
+Qed.
+
+Lemma body_KV_GetCharArraySize: semax_body Vprog Gprog f_KV_GetCharArraySize KV_GetCharArraySize_spec.
+Proof.
+  start_function.
+  unfold key_rep.
+  Intros.
+  forward_if (True); [forward; entailer! | assert_PROP (False) by entailer!; contradiction | ].
+  forward.
+  forward.
+  fold_keyrep.
+  entailer!.
+Qed.
